Update [only_affects] to only apply when result is ok. See msg.
This is necessary to be able to prove some properties about merging
blocks in series. However, this breaks some proofs that we had working
before. These will be fixed in future commits.

vale/code/lib/transformers/Vale.Transformers.BoundedInstructionEffects.fsti
@@ -39,7 +39,7 @@ let unchanged_except (exceptions:locations) (s1 s2:machine_state) :
     except [locs] unchanged. *)
 let only_affects (locs:locations) (f:st unit) : GTot Type0 =
   forall s. {:pattern unchanged_except locs s (run f s)} (
-    unchanged_except locs s (run f s)
+    (run f s).ms_ok ==> unchanged_except locs s (run f s)
   )
 
 (** [unchanged_at locs s1 s2] means the the value of any location in
