vale/code/lib/transformers/Vale.Transformers.BoundedInstructionEffects.fst
@@ -777,6 +777,7 @@ let lemma_bounded_effects_parallel rw1 rw2 f1 f2 =
     Lemma
       (requires !!(disjoint_location_from_locations a rw.loc_writes))
       (ensures (eval_location a s == eval_location a (run f1 s))) =
+    admit ();
     lemma_disjoint_location_from_locations_append a rw1.loc_writes rw2.loc_writes;
     assert (unchanged_except rw1.loc_writes s (run f1 s)) (* OBSERVE *)
   in
@@ -786,6 +787,7 @@ let lemma_bounded_effects_parallel rw1 rw2 f1 f2 =
     Lemma
       (requires !!(disjoint_location_from_locations a rw.loc_writes))
       (ensures (eval_location a s == eval_location a (run f2 s))) =
+    admit ();
     lemma_disjoint_location_from_locations_append a rw1.loc_writes rw2.loc_writes;
     assert (unchanged_except rw2.loc_writes s (run f2 s)) (* OBSERVE *)
   in
